Isabelle2/Max_Properties.thy
@@ -1,55 +1,98 @@
 section {* A few lemmas about Max *}
 
-theory Max_Properties 
-imports Main LinorderOption
+theory Max_Properties
+imports Main
 begin
-
-lemma Max_Max:
-  assumes "finite Xs" and "Union Xs \<noteq> {}" and "\<And> X . X \<in> Xs \<Longrightarrow> X \<noteq> {} \<and> finite X"
-  shows "Max (Max ` Xs) = Max (Union Xs)" (is "?A = ?B")
-  -- {* Is this of any use? Note that all subsets are required to be non-empty. *}
-nitpick[verbose, card 'a = 2, card "'a option" = 3, expect=none]
-proof -
-  have 0:"finite (Union Xs)" using assms(1,3) by auto
-  hence 1:"?B \<in> Union Xs"
-    by (metis Max_in assms(2))
-  have "finite (Max ` Xs)" by (metis assms(1) finite_imageI)
-  moreover have "Max ` Xs \<noteq> {}" using assms(2) by (metis Sup_empty image_is_empty) 
-  ultimately have 3:"?A \<in> (Max ` Xs)" and "\<And> x . x \<in> Max ` Xs \<Longrightarrow> x \<le> ?A"
-    by (metis Max_in, metis Max_ge \<open>finite (Max ` Xs)\<close>)
-  show ?thesis by (smt 1 3 Max_ge Max_mono Sup_upper UnionE 0 antisym assms(1,3) finite_imageI image_iff) 
-qed
-
-lemma Max_bot:"\<lbrakk>finite (S::'b::{linorder,order_bot} set); S \<noteq> {}; s \<in> S; Max S = bot\<rbrakk> \<Longrightarrow> s = bot"
-by (metis Max.coboundedI bot.extremum_uniqueI)
-
-lemma max_insert_none:
-  fixes S :: "'b::linorder option set"
-  assumes "S \<noteq> {}" and "finite S"
-  shows "Max (insert None S) = Max S"
-using bot_def Max_insert assms bot.extremum max_def by metis
-
-lemma Some_Max_commute:
-  fixes S::"'b::linorder set" assumes "S \<noteq> {}" and "finite S"
-  shows "Max (Some ` S) = Some (Max S)"
-proof -
-  have "mono (Some::('b::linorder \<Rightarrow> 'b option))" 
-  proof (auto simp add:mono_def)
-    fix x y :: "'b::linorder"
-    assume "x \<le> y"
-    thus "Some x \<le> Some y"
-      by (metis less_eq_def less_eq_o.simps(3)) 
-  qed
-  thus ?thesis
-  by (metis assms(1) assms(2) mono_Max_commute) 
-qed
 
 subsection {* Max by key *}
 
 definition max_by_key where
-  "max_by_key S f \<equiv>
-    let max_key = Max {f x | x . x \<in> S}
-    in SOME x . x \<in> S \<and> f x = max_key"
+  "max_by_key S f \<equiv> let max_key = Max {f x | x . x \<in> S} in SOME x . x \<in> S \<and> f x = max_key"
+
+definition max_by_key_2 where
+  -- {* Executable version *} 
+  "max_by_key_2 S f \<equiv> {x \<in> S . f x = Max (f ` S)}"
+
+lemma max_by_key_ne:assumes "S \<noteq> {}" and "finite S" shows "max_by_key_2 S f \<noteq> {}" using assms
+by (simp add:max_by_key_2_def) (metis (mono_tags, hide_lams) Max_in finite_imageI image_iff image_is_empty)
+
+export_code max_by_key_2 in SML
+value "max_by_key_2 {(1::nat,1),(0,3)} fst"
+
+lemma max_by_key_2_in_and_ge:
+  fixes S::"'b set" and x::'b 
+  assumes "finite S" and "x \<in> S" and "m \<in> max_by_key_2 S f"
+  shows "f x \<le> f m" and  "m \<in> S"
+proof -
+  from `finite S` have "finite (f ` S)" (is "finite ?keys") by simp
+  from `x \<in> S` have "?keys \<noteq> {}" by auto
+  have "f m = Max (f ` S)" by (metis (mono_tags, lifting) assms(3) max_by_key_2_def mem_Collect_eq) 
+  have "m \<in> S" by (metis (no_types, lifting) assms(3) max_by_key_2_def mem_Collect_eq) 
+  show "f x \<le> f m" and  "m \<in> S" by (simp add: \<open>f m = Max (f ` S)\<close> \<open>finite (f ` S)\<close> assms(2), simp add: \<open>m \<in> S\<close>)
+qed
+
+lemma in_and_ge_is_max_by_key_2: fixes S :: "'a set" and f :: "'a \<Rightarrow> ('b::linorder)"
+assumes "\<And> x . x \<in> S \<Longrightarrow> f x \<le> f m" and "m \<in> S" and "finite S"
+shows "m \<in> max_by_key_2 S f" using assms apply (simp add:max_by_key_2_def)
+proof -
+  assume a1: "\<And>x. x \<in> S \<Longrightarrow> f x \<le> f m"
+  assume a2: "m \<in> S"
+  assume a3: "finite S"
+  obtain aa :: "'b \<Rightarrow> ('a \<Rightarrow> 'b) \<Rightarrow> 'a set \<Rightarrow> 'a" where
+    f4: "\<forall>b. (\<forall>f A. b \<notin> f ` A \<or> aa b f A \<in> A \<and> b = f (aa b f A)) \<and> (\<forall>f A. (\<forall>a. (a::'a) \<notin> A \<or> b \<noteq> f a) \<or> b \<in> f ` A)"
+    by moura
+  have "finite (f ` S)"
+    using a3 by simp
+  then show "f m = Max (f ` S)"
+    using f4 a2 a1 by (metis (no_types) Max_ge Max_in equals0D order_class.order.antisym)
+qed 
+
+
+lemma max_by_key_2_subsets:
+  -- {* Lemma showing that computing max_by_key_2 in 2 steps, first computing the max per acceptor and then the max of those values, 
+  is the same thing as max_by_key_2. *}
+  fixes Ss :: "'a set set" and f :: "'a \<Rightarrow> ('b::linorder)" and S
+  assumes "\<And> S . S \<in> Ss \<Longrightarrow> finite S" and "finite Ss" and "S \<in> Ss" and "S \<noteq> {}"
+  shows "max_by_key_2 (Union {max_by_key_2 S f | S . S \<in> Ss \<and> S \<noteq> {}}) f = max_by_key_2 (Union Ss) f"
+proof -
+  def maxs \<equiv> "Union {max_by_key_2 S f | S . S \<in> Ss \<and> S \<noteq> {}}"
+  have 1:"finite maxs" 
+  proof -
+    have 1:"finite {max_by_key_2 S f | S . S \<in> Ss \<and> S \<noteq> {}}" using \<open>finite Ss\<close> by auto
+    have 2:"\<And> S . S \<in> Ss \<Longrightarrow> finite (max_by_key_2 S f)" using \<open>\<And> S . S \<in> Ss \<Longrightarrow> finite S\<close>  by (auto simp add:max_by_key_2_def)
+    show ?thesis using finite_Union[of "{max_by_key_2 S f | S . S \<in> Ss \<and> S \<noteq> {}}", OF 1] using 2 using CollectD maxs_def by blast
+  qed 
+  have 2:"maxs \<noteq> {}" 
+  proof -
+    have "max_by_key_2 S f \<noteq> {}" if "S \<in> Ss" and "S \<noteq> {}" for S using that 
+      by (simp add:max_by_key_2_def) (metis (mono_tags, lifting) Max_in assms(1) finite_imageI imageE image_is_empty)
+    thus ?thesis using assms(3) assms(4) using Sup_bot_conv(1) maxs_def mem_Collect_eq by auto 
+  qed
+  have 3:"finite (Union Ss)" using \<open>finite Ss\<close> and \<open>\<And> S . S \<in> Ss \<Longrightarrow> finite S\<close> by blast
+  { fix x assume a1:"x \<in> max_by_key_2 maxs f"
+    have a2:"x \<in> Union Ss" using a1 apply (simp add:max_by_key_2_def maxs_def) by (metis (no_types, lifting) mem_Collect_eq) 
+    have a3:"f x \<ge> f y" if "y \<in> Union Ss" for y
+    proof -
+      from that obtain S where "S \<in> Ss" and "y \<in> S" by auto
+      def M_S \<equiv> "max_by_key_2 S f"
+      have "M_S \<noteq> {}" using \<open>y \<in> S\<close> max_by_key_ne by (metis M_S_def \<open>S \<in> Ss\<close> assms(1) equals0D) 
+      have "f m_S \<ge> f y" if "m_S \<in> M_S" for m_S using \<open>S \<in> Ss\<close> \<open>y \<in> S\<close> assms(1) max_by_key_2_in_and_ge(1) that by (metis M_S_def) 
+      have "M_S \<subseteq> maxs" using \<open>S \<in> Ss\<close> \<open>y \<in> S\<close> by (auto simp add:M_S_def maxs_def)
+      have "f x \<ge> f m_S" if "m_S \<in> M_S" for m_S using a1 \<open>S \<in> Ss\<close> that by (metis "1" \<open>M_S \<subseteq> maxs\<close> max_by_key_2_in_and_ge(1) rev_subsetD) 
+      show ?thesis by (metis \<open>M_S \<noteq> {}\<close> \<open>\<And>m_S. m_S \<in> M_S \<Longrightarrow> f m_S \<le> f x\<close> \<open>\<And>m_S. m_S \<in> M_S \<Longrightarrow> f y \<le> f m_S\<close> ex_in_conv order_trans)
+    qed
+    note a2 a3 }
+  hence 4:"max_by_key_2 maxs f \<subseteq> max_by_key_2 (Union Ss) f" by (metis "3" in_and_ge_is_max_by_key_2 subsetI)
+  { fix x assume a1:"x \<in> max_by_key_2 (Union Ss) f"
+    obtain S where "S \<in> Ss" and "x \<in> S" by (metis "3" Union_iff a1 assms(3) assms(4) ex_in_conv max_by_key_2_in_and_ge(2))
+    have "f x \<ge> f y" if "y \<in> S'" and "S' \<in> Ss" for y S' by (metis "3" UnionI a1 max_by_key_2_in_and_ge(1) that(1) that(2)) 
+    have "x \<in> max_by_key_2 S f" by (metis \<open>S \<in> Ss\<close> \<open>\<And>y S'. \<lbrakk>y \<in> S'; S' \<in> Ss\<rbrakk> \<Longrightarrow> f y \<le> f x\<close> \<open>x \<in> S\<close> assms(1) in_and_ge_is_max_by_key_2)
+    have a2:"x \<in> maxs" apply (simp add:maxs_def) by (metis \<open>S \<in> Ss\<close> \<open>x \<in> S\<close> \<open>x \<in> max_by_key_2 S f\<close> equals0D)
+    have a3:"f x \<ge> f y" if "y \<in> maxs" for y using that apply (simp add:maxs_def) by (metis "3" Union_iff a1 assms(1) bot.extremum_uniqueI max_by_key_2_in_and_ge(1) max_by_key_2_in_and_ge(2) subset_emptyI) 
+    note a2 a3 }
+  hence 5:"max_by_key_2 (Union Ss) f \<subseteq> max_by_key_2 maxs f" by (metis "1" in_and_ge_is_max_by_key_2 subsetI) 
+  from 4 5 show ?thesis using maxs_def set_eq_subset by blast
+qed
 
 lemma max_by_key_in_and_ge: fixes S::"'b set" and x::'b assumes "finite S" and "x \<in> S"
   shows "f x \<le> f (max_by_key S f)" and "max_by_key S f \<in> S"
@@ -66,14 +109,14 @@ proof -
   show "f x \<le> f (max_by_key S f)" and "max_by_key S f \<in> S" 
     apply (auto simp add:max_by_key_def)
     using Max.coboundedI \<open>f (SOME x. x \<in> S \<and> f x = Max {f x |x. x \<in> S}) = Max {f x |x. x \<in> S}\<close> \<open>finite {f x |x. x \<in> S}\<close> assms(2) apply auto[1]
-    using \<open>(SOME x. x \<in> S \<and> f x = Max {f x |x. x \<in> S}) \<in> S\<close> by blast 
+    using \<open>(SOME x. x \<in> S \<and> f x = Max {f x |x. x \<in> S}) \<in> S\<close> by blast
 qed
 
 lemma in_and_ge_is_max_by_key: fixes S :: "'a set" and f :: "'a \<Rightarrow> ('b::linorder)"
   assumes "\<And> x . x \<in> S \<Longrightarrow> f x \<le> f m" and "m \<in> S" and "finite S" and "\<And> x y . \<lbrakk>x \<in> S; y \<in> S; x \<noteq> y\<rbrakk> \<Longrightarrow> f x \<noteq> f y"
   shows "m = max_by_key S f" 
 nitpick[verbose,  card 'a = 4, card 'b =6, card "'b option" = 30, expect = none]
-proof (rule ccontr) 
+proof (rule ccontr)
   assume "m \<noteq> max_by_key S f" (is "m \<noteq> ?m'")
   have "\<And> x . x \<in> S \<Longrightarrow> f x \<le> f ?m'" and "?m' \<in> S"
     apply (metis assms(3) max_by_key_in_and_ge(1)) by (metis assms(2) assms(3) max_by_key_in_and_ge(2)) 
@@ -98,12 +141,7 @@ proof -
     have 2:"\<And> x . x \<in> S \<Longrightarrow> f x \<le> f (max_by_key S f)" by (metis \<open>S \<in> Ss\<close> assms(1) max_by_key_in_and_ge(1))
     note 1 2 }
   note 1 = this
-  { { fix x assume "x \<in> ?maxs"
-        obtain S where "S \<in> Ss" and "S \<noteq> {}" and "x = max_by_key S f" using \<open>x \<in> {max_by_key S f |S. S \<in> Ss \<and> S \<noteq> {}}\<close> by blast 
-        with 1 have "x \<in> S" by (meson all_not_in_conv assms(1) max_by_key_in_and_ge(2))
-        hence "x \<in> Union Ss" using \<open>S \<in> Ss\<close> by blast }
-      note 4 = this
-      have 2:"max_by_key ?maxs f \<in> ?maxs" and 3:"\<And> m . m \<in> ?maxs \<Longrightarrow> f m \<le> f (max_by_key ?maxs f)"
+  { have 2:"max_by_key ?maxs f \<in> ?maxs" and 3:"\<And> m . m \<in> ?maxs \<Longrightarrow> f m \<le> f (max_by_key ?maxs f)"
         apply (metis (no_types, lifting) \<open>finite {max_by_key S f |S. S \<in> Ss \<and> S \<noteq> {}}\<close> \<open>{max_by_key S f |S. S \<in> Ss \<and> S \<noteq> {}} \<noteq> {}\<close> ex_in_conv max_by_key_in_and_ge(2))
         by (metis (no_types, lifting) \<open>finite {max_by_key S f |S. S \<in> Ss \<and> S \<noteq> {}}\<close> max_by_key_in_and_ge(1))
     note 2 3 }
@@ -112,6 +150,43 @@ proof -
     have 4:"\<And> x . x \<in> Union Ss \<Longrightarrow> f x \<le> f (max_by_key ?maxs f)"  using "1"(2) "2"(2) apply auto by (metis (no_types, lifting) empty_iff order_trans) 
     note 3 4 }
   thus ?thesis using in_and_ge_is_max_by_key[where ?S="Union Ss" and ?f=f] by (metis (mono_tags, lifting) \<open>finite (\<Union>Ss)\<close> assms(5)) 
+qed
+
+subsection {* Other properties *}
+text {* Used anywhere? *}
+
+lemma Max_Max:
+  assumes "finite Xs" and "Union Xs \<noteq> {}" and "\<And> X . X \<in> Xs \<Longrightarrow> X \<noteq> {} \<and> finite X"
+  shows "Max (Max ` Xs) = Max (Union Xs)" (is "?A = ?B")
+  -- {* Is this of any use? Note that all subsets are required to be non-empty. *}
+nitpick[verbose, card 'a = 2, card "'a option" = 3, expect=none]
+proof -
+  have 0:"finite (Union Xs)" using assms(1,3) by auto
+  hence 1:"?B \<in> Union Xs"
+    by (metis Max_in assms(2))
+  have "finite (Max ` Xs)" by (metis assms(1) finite_imageI)
+  moreover have "Max ` Xs \<noteq> {}" using assms(2) by (metis Sup_empty image_is_empty) 
+  ultimately have 3:"?A \<in> (Max ` Xs)" and "\<And> x . x \<in> Max ` Xs \<Longrightarrow> x \<le> ?A"
+    by (metis Max_in, metis Max_ge \<open>finite (Max ` Xs)\<close>)
+  show ?thesis by (smt 1 3 Max_ge Max_mono Sup_upper UnionE 0 antisym assms(1,3) finite_imageI image_iff) 
+qed
+
+lemma Max_bot:"\<lbrakk>finite (S::'b::{linorder,order_bot} set); S \<noteq> {}; s \<in> S; Max S = bot\<rbrakk> \<Longrightarrow> s = bot"
+by (metis Max.coboundedI bot.extremum_uniqueI)
+
+lemma max_by_key_in:
+  assumes "finite S" and "S \<noteq> {}" and "max_by_key_2 S f \<noteq> {}" and "m = max_by_key S f"
+  shows "m \<in> max_by_key_2 S f" using assms
+proof-
+  {
+    assume 0:"m \<notin> max_by_key_2 S f"
+    have 1:"m \<in> S" using assms(1,2,4) by (meson all_not_in_conv max_by_key_in_and_ge(2))
+    have 2:"f m = Max {f x | x . x \<in> S}" using 0 1 assms(1,4) 
+      by (metis (no_types, lifting) in_and_ge_is_max_by_key_2 max_by_key_in_and_ge(1))
+    hence "False" using 0 1 assms(1,4)  max_by_key_2_def
+      by (metis (no_types, lifting) in_and_ge_is_max_by_key_2 max_by_key_in_and_ge(1))
+  }
+  thus ?thesis by blast
 qed
 
 end
